\documentclass[10pt,a4paper]{article}
\usepackage{amsmath, amssymb, amsthm}
%加這個就可以設定字體
\usepackage{fontspec}
\usepackage{xkeyval} %MikTeX 2.9 版本相容有誤, 以此修正
%使用xeCJK，其他的還有CJK或是xCJK
\usepackage{xeCJK}
%設定英文字型，不設的話就會使用預設的字型
%\setmainfont{Times New Roman}
%設定中英文的字型
%字型的設定可以使用系統內的字型，而不用像以前一樣另外安裝
%\setCJKmainfont{文泉驛微米黑}
\setCJKmainfont{WenQuanYi Micro Hei}
\setCJKfamilyfont{lh}{LiHei Pro}
\newcommand{\LiHei}{\CJKfamily{lh}}
%中文自動換行
\XeTeXlinebreaklocale "zh"
%文字的彈性間距
\XeTeXlinebreakskip = 0pt plus 1pt
%設定段落之間的距離
\setlength{\parskip}{0.3cm}
%設定行距
%\linespread{1.5}\selectfont

%先暫時用水泥字型，如果任何人看不下去就改吧XD
\usepackage[T1]{fontenc}
\usepackage{concmath}
%\usepackage{mathptmx} %Times

\newcounter{theProblemCounter}
\newtheorem{problem}[theProblemCounter]{Problem}

\begin{document}
\title{{\fontspec{Copperplate Gothic Bold}Geometry Homework 5}}
%\title{{\fontspec{Copperplate}Geometry Homework 5}}
\author{{\it{B96201044}} {\LiHei 黃上恩}, {\it{B98901182}} {\LiHei 時丕勳}, {\it{K0020100x}} {\LiHei 劉士瑋}}
\date{\today}
\maketitle

\newcommand{\bx}{\mathbb{X}}
%第一題
\setcounter{theProblemCounter}{0}
\begin{problem}[Ex P151 2]
Show that if a surface is tangent to a plane along a curve, then the points of this curve are either parabolic or planar.
\end{problem}
\begin{proof}
Assume that the curve is $\gamma(s)$, then along this curve, $N(\gamma(s))$ is perpendicular to the plane, so it is constant.\\
At point $\gamma(s)$, $[dN](\gamma'(s))=\left(\frac{d N(\gamma(t))}{dt}\right)_{t=s}=0$, so $\gamma'(s)$ is one of the principal direction of the surface at $\gamma(s)$, and it's associated principal curvature is $0$.\\
So the gaussian curvature of the surface at $\gamma(s)$ is $K=0$, and this means that the point $\gamma(s)$ is either parabolic or planar.
\end{proof}

%第三題
\setcounter{theProblemCounter}{2}
\begin{problem}[Ex P151 3]
\begin{enumerate}
\item[]
\item[(a)] Let $C\subset S$ be a regular curve on a surface $S$ with Gaussian curvature $K > 0$. Show that the curvature $\kappa$ of $C$ at $p$ satisfies \[ \kappa\ge \min(|\kappa_1|, |\kappa_2|),\] where $\kappa_1, \kappa_2$ are the principal curvatures of $S$ at $p$.
\item[(b)] 為什麼上一小題需要 $\kappa>0$ 的條件，$\kappa\ge 0$ 不可以嗎？ %好像的確是想說 \kappa 耶(?)
\end{enumerate}
\end{problem}
\begin{proof}
\begin{enumerate}
\item[(a)]
\begin{align*}
\kappa&\ge |\kappa_n|\\
&=|\kappa_1\cos^2\theta+\kappa_2\sin^2\theta|\\
&=|\kappa_1|\cos^2\theta+|\kappa_2|\sin^2\theta (\because\kappa_1, \kappa_2\textrm{ has equal sign.})\\
&\ge \min(|\kappa_1|, |\kappa_2|)(\cos^2\theta+\sin^2\theta)\\
&=\min(|\kappa_1|, |\kappa_2|)
\end{align*}
\item[(b)]
% 若 $K=0$, 則 $\kappa_1, \kappa_2$ 中必定要有一個為零, 則 $\min(|\kappa_1|, |\kappa_2|)=0$, 而 $\kappa\ge 0$ 顯然成立. 故條件亦可改為 $K\ge 0$.
上一小題的證明中並沒有用到 $\kappa\neq 0$ 或是 $K\neq 0$.
\end{enumerate}
\end{proof}

%第七題
\setcounter{theProblemCounter}{6}
\begin{problem}
\begin{enumerate}
\item[]
\item[(a)] $T_\lambda$ 是縮放 $\lambda$ 倍的映射，$\lambda>0$。$\mathbb{X}:\Omega\to \mathbb{R}^3$ regular surface。討論 $T_\lambda\circ \mathbb{X}:\Omega\to\mathbb{R}^3$ 上對應點 $\kappa_n, H, K$ 的變化。
\item[(b)] $\mathbb{X}:\begin{array}{c}\Omega\\(u,v)\end{array}\to \mathbb{R}^3$，若定義 $\overline{\mathbb{X}}(u, v)= \mathbb{X}(v, u)$(因此 $N$ 轉向)。討論 $\overline{\mathbb{X}}(\Omega)$ 上相對應點的 $\kappa_n, H, K$ 變化。 %這顯然是題目打錯
\end{enumerate}
\end{problem}
\begin{proof}
\begin{enumerate}
\item[(a)]
不妨設縮放中心為原點. 令 $\overline{\mathbb{X}}=T_\lambda\circ \mathbb{X}$, 所以 $\overline{\mathbb{X}}(u,v)=\lambda\mathbb{X}(u,v)$.\\
\begin{align*}
\overline{\mathbb{X}}_u&=\lambda\mathbb{X}_u\\
\overline{\mathbb{X}}_v&=\lambda\mathbb{X}_v\\
N_{\overline{\mathbb{X}}}&=\frac{\overline{\mathbb{X}}_u\times\overline{\mathbb{X}}_v}{|\overline{\mathbb{X}}_u\times\overline{\mathbb{X}}_v|}\\
&=\frac{\lambda^2\mathbb{X}_u\times\mathbb{X}_v}{\lambda^2|\mathbb{X}_u\times\mathbb{X}_v|}\\
&=\frac{\mathbb{X}_u\times\mathbb{X}_v}{|\mathbb{X}_u\times\mathbb{X}_v|}\\
&=N_{\mathbb{X}}\\
\end{align*}
\begin{align*}
E_{\overline{\mathbb{X}}} &= \langle \overline{\mathbb{X}}_u, \overline{\mathbb{X}}_u\rangle\\
&= \lambda^2\langle \mathbb{X}_u, \mathbb{X}_u\rangle\\
&= \lambda^2 E_{\mathbb{X}}\\
F_{\overline{\mathbb{X}}} &= \langle \overline{\mathbb{X}}_u, \overline{\mathbb{X}}_v\rangle\\
&= \lambda^2\langle \mathbb{X}_u, \mathbb{X}_v\rangle\\
&= \lambda^2 F_{\mathbb{X}}\\
G_{\overline{\mathbb{X}}} &= \langle \overline{\mathbb{X}}_v, \overline{\mathbb{X}}_v\rangle\\
&= \lambda^2\langle \mathbb{X}_v, \mathbb{X}_v\rangle\\
&= \lambda^2 G_{\mathbb{X}}\\
\end{align*}
\begin{align*}
\overline{\mathbb{X}}_{uu}&=\lambda\mathbb{X}_{uu}\\
\overline{\mathbb{X}}_{uv}&=\lambda\mathbb{X}_{uv}\\
\overline{\mathbb{X}}_{vv}&=\lambda\mathbb{X}_{vv}\\
e_{\overline{\mathbb{X}}} &= \langle N_{\overline{\mathbb{X}}}, \overline{\mathbb{X}}_{uu}\rangle\\
&= \lambda \langle N_{\mathbb{X}}, \mathbb{X}_{uu}\rangle\\
&= \lambda e_{\mathbb{X}}\\
f_{\overline{\mathbb{X}}} &= \langle N_{\overline{\mathbb{X}}}, \overline{\mathbb{X}}_{uv}\rangle\\
&= \lambda \langle N_{\mathbb{X}}, \mathbb{X}_{uv}\rangle\\
&= \lambda f_{\mathbb{X}}\\
g_{\overline{\mathbb{X}}} &= \langle N_{\overline{\mathbb{X}}}, \overline{\mathbb{X}}_{vv}\rangle\\
&= \lambda \langle N_{\mathbb{X}}, \mathbb{X}_{vv}\rangle\\
&= \lambda g_{\mathbb{X}}\\
\end{align*}
\begin{align*}
[-dN]_{\overline{\mathbb{X}}} &= \left[\begin{array}{cc}E_{\overline{\mathbb{X}}} & F_{\overline{\mathbb{X}}} \\ F_{\overline{\mathbb{X}}} & G_{\overline{\mathbb{X}}}\end{array}\right]^{-1}\left[\begin{array}{cc}e_{\overline{\mathbb{X}}} & f_{\overline{\mathbb{X}}} \\ f_{\overline{\mathbb{X}}} & g_{\overline{\mathbb{X}}}\end{array}\right]\\
&= \frac{1}{\lambda^2}\left[\begin{array}{cc}E_{\mathbb{X}} & F_{\mathbb{X}} \\ F_{\mathbb{X}} & G_{\mathbb{X}}\end{array}\right]^{-1}\left[\begin{array}{cc}e_{\mathbb{X}} & f_{\mathbb{X}} \\ f_{\mathbb{X}} & g_{\mathbb{X}}\end{array}\right]\\
&=\frac{1}{\lambda^2}[-dN]_{\mathbb{X}}\\
\rightarrow \kappa_{n\overline{\mathbb{X}}} &= \frac{1}{\lambda^2}\kappa_{n\mathbb{X}}\\
K_{\overline{\mathbb{X}}} &= \frac{1}{\lambda^4}K_{\mathbb{X}}\\
H_{\overline{\mathbb{X}}} &= \frac{1}{\lambda^2}H_{\mathbb{X}}\\
\end{align*}
\item[(b)]
\begin{align*}
\overline{\mathbb{X}}_u&=\mathbb{X}_v\\
\overline{\mathbb{X}}_v&=\mathbb{X}_u\\
N_{\overline{\mathbb{X}}}&=\frac{\overline{\mathbb{X}}_u\times\overline{\mathbb{X}}_v}{|\overline{\mathbb{X}}_u\times\overline{\mathbb{X}}_v|}\\
&=\frac{\mathbb{X}_v\times\mathbb{X}_u}{|\mathbb{X}_u\times\mathbb{X}_v|}\\
&=-N_{\mathbb{X}}\\
\end{align*}
\begin{align*}
E_{\overline{\mathbb{X}}} &= \langle \overline{\mathbb{X}}_u, \overline{\mathbb{X}}_u\rangle\\
&= \langle \mathbb{X}_v, \mathbb{X}_v\rangle\\
&= G_{\mathbb{X}}\\
F_{\overline{\mathbb{X}}} &= \langle \overline{\mathbb{X}}_u, \overline{\mathbb{X}}_v\rangle\\
&= \langle \mathbb{X}_v, \mathbb{X}_u\rangle\\
&= F_{\mathbb{X}}\\
G_{\overline{\mathbb{X}}} &= \langle \overline{\mathbb{X}}_v, \overline{\mathbb{X}}_v\rangle\\
&= \langle \mathbb{X}_u, \mathbb{X}_u\rangle\\
&= E_{\mathbb{X}}\\
\end{align*}
\begin{align*}
\overline{\mathbb{X}}_{uu}&=\mathbb{X}_{vv}\\
\overline{\mathbb{X}}_{uv}&=\mathbb{X}_{uv}\\
\overline{\mathbb{X}}_{vv}&=\mathbb{X}_{uu}\\
e_{\overline{\mathbb{X}}} &= \langle N_{\overline{\mathbb{X}}}, \overline{\mathbb{X}}_{uu}\rangle\\
&= \langle -N_{\mathbb{X}}, \mathbb{X}_{vv}\rangle\\
&= -g_{\mathbb{X}}\\
f_{\overline{\mathbb{X}}} &= \langle N_{\overline{\mathbb{X}}}, \overline{\mathbb{X}}_{uv}\rangle\\
&= \langle -N_{\mathbb{X}}, \mathbb{X}_{uv}\rangle\\
&= -f_{\mathbb{X}}\\
g_{\overline{\mathbb{X}}} &= \langle N_{\overline{\mathbb{X}}}, \overline{\mathbb{X}}_{vv}\rangle\\
&= \langle -N_{\mathbb{X}}, \mathbb{X}_{uu}\rangle\\
&= -e_{\mathbb{X}}\\
\end{align*}
\begin{align*}
[-dN]_{\overline{\mathbb{X}}} &= \left[\begin{array}{cc}E_{\overline{\mathbb{X}}} & F_{\overline{\mathbb{X}}} \\ F_{\overline{\mathbb{X}}} & G_{\overline{\mathbb{X}}}\end{array}\right]^{-1}\left[\begin{array}{cc}e_{\overline{\mathbb{X}}} & f_{\overline{\mathbb{X}}} \\ f_{\overline{\mathbb{X}}} & g_{\overline{\mathbb{X}}}\end{array}\right]\\
&= -\left[\begin{array}{cc}G_{\mathbb{X}} & F_{\mathbb{X}} \\ F_{\mathbb{X}} & E_{\mathbb{X}}\end{array}\right]^{-1}\left[\begin{array}{cc}g_{\mathbb{X}} & f_{\mathbb{X}} \\ f_{\mathbb{X}} & e_{\mathbb{X}}\end{array}\right]\\
&=-\begin{bmatrix}0&1\\1&0\end{bmatrix}[-dN]_{\mathbb{X}}\begin{bmatrix}0&1\\1&0\end{bmatrix}\\
\rightarrow \kappa_{n\overline{\mathbb{X}}} &= -\kappa_{n\mathbb{X}}\\
K_{\overline{\mathbb{X}}} &= K_{\mathbb{X}}\\
H_{\overline{\mathbb{X}}} &= -H_{\mathbb{X}}\\
\end{align*}
\end{enumerate}
\end{proof}

%第九題
\setcounter{theProblemCounter}{8}
\begin{problem}[旋轉面]
$\mathbb{X}(u, v)=(f(u)\cos v, f(u)\sin v, g(u))$，$f>0$ \begin{enumerate}
\item[(a)] 計算其 $e, f, g, H, K$
\item[(b)] 討論其 principal direction 與 principal curvature $K_1, K_2$。
\end{enumerate}
\end{problem}
\begin{proof}
To avoid the notational ambiguity, let $\mathbb{X}(u, v)=(s(u)\cos v, s(u)\sin v, t(u))$, and that $s>0$. \begin{enumerate}
\item[(a)] We have
\begin{align*}
\mathbb{X}_u &= (s'(u)\cos v, s'(u)\sin v, t'(u)); \\
\mathbb{X}_v &= (-s(u)\sin v, s(u)\cos v, 0); \\
E &= \langle \mathbb{X}_u, \mathbb{X}_u\rangle = s'(u)^2 + t'(u)^2 \\
F &= \langle \mathbb{X}_u, \mathbb{X}_v\rangle = 0 \\
G &= \langle \mathbb{X}_v, \mathbb{X}_v\rangle = s(u)^2 \\
\mathbb{X}_{uu} &= (s''(u)\cos v, s''(u)\sin v, t''(u)); \\
\mathbb{X}_{uv} &= (-s'(u)\sin v, s'(u)\cos v, 0); \\
\mathbb{X}_{vv} &= (-s(u)\cos v, -s(u)\sin v, 0); \\
N &= \frac{\mathbb{X}_u \times \mathbb{X}_v}{|\mathbb{X}_u \times \mathbb{X}_v|} = \frac{(-t'(u)s(u)\cos v, -t'(u)s(u)\sin v, s'(u)s(u))}{\sqrt{t'(u)^2s(u)^2 + s'(u)^2s(u)^2}} \\
  &= \frac{(-t'(u)\cos v, -t'(u)\sin v, s'(u))}{\sqrt{t'(u)^2 + s'(u)^2}}; \\
e &= \langle N, \mathbb{X}_{uu}\rangle = \frac{-s''(u)t'(u) + t''(u)s'(u)}{\sqrt{t'(u)^2 + s'(u)^2}} \\
f &= \langle N, \mathbb{X}_{uv}\rangle = 0 \\
g &= \langle N, \mathbb{X}_{vv}\rangle = \frac{s(u)t'(u)}{\sqrt{t'(u)^2 + s'(u)^2}} \\
-dN^T &= \left[\begin{array}{cc}e & f \\ f & g\end{array}\right]\left[\begin{array}{cc}E & F \\ F & G\end{array}\right]^{-1} = \frac 1{EG - F^2}\left[\begin{array}{cc}e & f \\ f & g\end{array}\right]\left[\begin{array}{cc}G & -F \\ -F & E\end{array}\right] = \left[\begin{array}{cc}e/E & 0 \\ 0 & g/G\end{array}\right]\\
K &= \det(-dN) = \frac{eg}{EG} \\
H &= \frac 12\text{tr}(-dN) = \frac{eG + gE}{2EG}
\end{align*}
\item[(b)]
Since $-dN$ is already a diagonal matrix, clearly, \begin{align*}
K_1 &= e/E; \\
K_2 &= g/G; \\
V_1 &= \mathbb{X}_u; \\
V_2 &= \mathbb{X}_v;
\end{align*}
\end{enumerate}
\end{proof}

%第十題
\setcounter{theProblemCounter}{9}
\begin{problem}[管面]
$\mathbb{X}(s,\theta) = \gamma(s)+\cos\theta\vec{n}(s) + \sin\theta\vec{b}(s)$, $0<\kappa < 1$
\begin{enumerate}
\item[(a)] 計算其 $e, f, g, H, K$
\item[(b)] 討論曲面上 $K$ 的分佈。
\end{enumerate}
\end{problem}
\begin{proof}
\begin{enumerate}
\item[(a)] 
Let $\vec{t}(s), \vec{n}(s), \vec{b}(s)$ be the basis, and $\gamma(0)$ be the origin.
\begin{align*}
\mathbb{X}_{s} &= (1 - \kappa\cos\theta, \tau\sin\theta, -\tau\cos\theta); \\
\mathbb{X}_{\theta} &= (0, -\sin\theta, \cos\theta); \\
N &= \frac{\mathbb{X}_{s} \times \mathbb{X}_{\theta}}{|\mathbb{X}_{s} \times \mathbb{X}_{\theta}|} = \frac{(0, (\kappa\cos\theta - 1)\cos\theta, (\kappa\cos\theta - 1)\sin\theta)}{|\kappa\cos\theta - 1|} \\
  &= (0, -\cos\theta, -\sin\theta); \quad\text{(since $\kappa< 1$)} \\
\mathbb{X}_{ss} &= (-\sin\theta\kappa\tau - \kappa'\cos\theta, \kappa + \cos\theta(-\kappa^2 - \tau^2) + \tau'\sin\theta, -\sin\theta\tau^2 - \tau'\cos\theta); \\
\mathbb{X}_{s\theta} &= (1 + \kappa\sin\theta, \tau\cos\theta, \tau\sin\theta); \\
\mathbb{X}_{\theta\theta} &= (0, -\cos\theta, -\sin\theta); \\
e &= -\kappa\cos\theta + \cos^2\theta(\kappa^2 + \tau^2) + \tau^2\sin^2\theta = -\kappa\cos\theta + \kappa^2\cos^2\theta + \tau^2; \\
f &= -\tau; \\
g &= 1; \\
dN(\mathbb{X}_{s}) &= N_{s} = (\kappa\cos\theta, -\tau\sin\theta, \tau\cos\theta) = \frac{\kappa}{1-\kappa}\mathbb{X}_{s} + \frac{\tau}{1-\kappa}\mathbb{X}_{\theta}; \\
dN(\mathbb{X}_{\theta}) &= N_{\theta} = (0, \sin\theta, -\cos\theta) = -\mathbb{X}_{\theta}; \\
[-dN] &= \left[\begin{array}{cc} \frac{-\kappa\cos\theta}{1-\kappa\cos\theta} & 0 \\ \frac{-\tau}{1-\kappa\cos\theta}  & 1\end{array}\right] \\
\kappa_1 &= \frac{-\kappa\cos\theta}{1-\kappa\cos\theta}; \\
\kappa_2 &= 1; \\
K &= \frac{-\kappa\cos\theta}{1-\kappa\cos\theta}; \\
H &= \frac{1-2\kappa\cos\theta}{1-\kappa\cos\theta}.
\end{align*}
\item[(b)] 
\begin{align*}
K &= \frac{-\kappa\cos\theta}{1-\kappa\cos\theta};\\
&= 1-\frac{1}{1-\kappa\cos\theta};\\
\end{align*}
Since $0<\kappa<1$, $K$ has a maximum of $\frac{\kappa}{1+\kappa}$ when $\cos\theta = -1$, i.e. $\theta = \pi$.\\
$K=0$ when $\cos\theta = 0$, i.e. $\theta = \frac{\pi}{2},\frac{3\pi}{2}$.\\
$K$ has a minimum of $\frac{-\kappa}{1-\kappa}$ when $\cos\theta = 1$, i.e. $\theta = 0$.
\end{enumerate}
\end{proof}
\end{document}
